fix miniparse stubs

examples/miniparse/bench/MiniStub.fst
@@ -10,4 +10,4 @@ module T = FStar.Tactics
 #set-options "--log_queries"
 
 let p__SUFFIX__ = T.synth_by_tactic (fun () -> gen_enum_parser T.__POLICY__ (`test))
-let q__SUFFIX__ = T.synth_by_tactic (fun () -> gen_parser32 T.__POLICY__ (`p))
+let q__SUFFIX__ = T.synth_by_tactic (fun () -> gen_parser_impl T.__POLICY__)
