examples/miniparse/bench/MiniStub.fsti
@@ -4,5 +4,5 @@ open MiniParse.Impl.Base
 type test = __CTORS__
 
 noextract
-val p__SUFFIX__ : parser test
-val q__SUFFIX__ : parser32 p
+val p__SUFFIX__ : parser_spec test
+val q__SUFFIX__ : parser_impl p__SUFFIX__
